\documentclass{article}
\input{preamble.tex}

% Title
\title{MATH 201}
\subtitle{Linear Algebra and Vector Geometry}
\author{Open Courseware}
\kind{Lecture \#5 \hfill \today}
\date{\today}

% Document
\begin{document}

% front matter
\mnfrontpage
\tableofcontents

% main matter
\section{Operations of Matrices}

\begin{definition}[Matrix]
    It is basically a table of numbers arranged in rows and columns.
\end{definition}

\begin{example}[Matrix]
    \[
        A_{2\times3} =
        \begin{bmatrix}
            1 & 2 & 3 \\
            4 & 5 & 6
        \end{bmatrix}
    .\] 
\end{example}

If we have a matrix in which the number of rows is equal to the number of columns, then it is called a square matrix.

\begin{note}
    For symbol notation, we usually use the capital letters for matrices and the small ones for the entries:
    \[
        A_{m\times n} =
        \begin{bmatrix} 
            a_{11} & a_{12} & \cdots & a_{1n} \\
            a_{21} & a_{22} & \cdots & a_{2n} \\
            \vdots & \vdots & \ddots & \vdots \\
            a_{m1} & a_{m2} & \cdots & a_{mn}
        \end{bmatrix} 
    .\] 
\end{note}

\subsection{Addition of Matrices}

We can only add two matrices if they have the same dimensions. 

\begin{example}
    \[
        \begin{bmatrix}
            1 & 2 & 3 \\
            4 & 5 & 6
        \end{bmatrix}
        + 
        \begin{bmatrix}
            1 & 2 & 3 \\
            4 & 5 & 6
        \end{bmatrix}
        =
        \begin{bmatrix}
            2 & 4 & 6 \\
            8 & 10 & 12
        \end{bmatrix}
    .\]
\end{example}

\subsection{Scalar Multiplication of a Matrix}

\[
    k
    \begin{bmatrix} 
        a_{11} & a_{12} \\
        a_{21} & a_{22}
    \end{bmatrix} 
    =
    \begin{bmatrix} 
        ka_{11} & ka_{12} \\
        ka_{21} & ka_{22}
    \end{bmatrix}
.\] 

\begin{example}
    \[
        2
        \begin{bmatrix} 
            1 & 2 \\
            3 & 4
        \end{bmatrix} 
        =
        \begin{bmatrix} 
            2 & 4 \\
            6 & 8
        \end{bmatrix}
    .\]
\end{example}

\subsection{Multiplication of Matrices}

To be able to multiply two matrices, the number of columns of the first matrix must be equal to the number of rows of the second matrix.

\[
    A_{m\times n} \times B_{n\times p} = C_{m\times p}
.\] 

\begin{example}[Compute AB]
    \[
        A =
        \begin{bmatrix}
            2 & 3 \\
            1 & -5
        \end{bmatrix},
        B =
        \begin{bmatrix}
            4 & 3 & 6 \\
            1 & -2 & 3
        \end{bmatrix}
    \] 
    \begin{align*}
        AB &= 
        \begin{bmatrix}
            2 & 3 \\
            1 & -5
        \end{bmatrix}
        \begin{bmatrix}
            4 & 3 & 6 \\
            1 & -2 & 3
        \end{bmatrix}\\
           &=
        \begin{bmatrix}
            2 \times 4 + 3 \times 1 & 2 \times 3 + 3 \times (-2) & 2 \times 6 + 3 \times 3 \\
            1 \times 4 + (-5) \times 1 & 1 \times 3 + (-5) \times (-2) & 1 \times 6 + (-5) \times 3
        \end{bmatrix}\\
           &=
        \begin{bmatrix}
            10 & -4 & 18 \\
            1 & 11 & 3
        \end{bmatrix}
    .\end{align*}
\end{example}

\subsubsection{Row-vector rule}%
\[
    (AB)_{ij} = \text{row}_{i}(A) \cdot \vec{b}_j
.\] 

\begin{example}
    If we want to find the 3rd element in the 1st row of $AB$, we dot product $A$'s 1st row with $B$'s 3rd column.
\end{example}

\hh

For $A_{m\times n}$ and $B_{n\times p}$,
\begin{itemize}
    \item $AB$ exist if $n = p$.
    \item $AB$ exist if $m\times q$ matrix.
    \item $(AB)_{ij} = \sum_{k=1}^n a_{ik}b_{kj}$.
\end{itemize}

\begin{example}[Find $AB$ and $BA$]
    \[
        A =
        \begin{bmatrix}
            1&3\\
            2&-1
        \end{bmatrix},
        B =
        \begin{bmatrix}
            2&-1\\
            0&2
        \end{bmatrix}
    \] 
    \begin{align*}
        AB &= 
        \begin{bmatrix}
            1&3\\
            2&-1
        \end{bmatrix}
        \begin{bmatrix}
            2&-1\\
            0&2
        \end{bmatrix}
        =
        \begin{bmatrix}
            2 & 5 \\
            4 & -3
        \end{bmatrix}\\
        BA &=
        \begin{bmatrix}
            2&-1\\
            0&2
        \end{bmatrix}
        \begin{bmatrix}
            1&3\\
            2&-1
        \end{bmatrix}
        =
        \begin{bmatrix}
            0&7\\
            4&-2
        \end{bmatrix}
    .\end{align*}
\end{example}

\begin{note}
    \[
        AB \neq BA
    .\] 
\end{note}

\hh\newpage

\begin{example}[$AB=0$ while $A \neq 0$ and $B\neq 0$]
    \[
        AB = 
        \begin{bmatrix} 1&3\\2&6 \end{bmatrix}
        \begin{bmatrix} 3&6\\-1&-2 \end{bmatrix} 
        =
        \begin{bmatrix} 0&0\\0&0 \end{bmatrix} 
    .\] 
\end{example}

\begin{example}[Find $(A+B)^2$, $A^2+2AB+B^2$]
    \[
        A =
        \begin{bmatrix}
            1&3\\
            2&-1
        \end{bmatrix},
        B =
        \begin{bmatrix}
            2&-1\\
            0&2
        \end{bmatrix}
    .\] 
    \begin{align*}
        (A+B)^2 &= (A+B)(A+B)\\
                &= 
        \begin{bmatrix}
            1&3\\
            2&-1
        \end{bmatrix}
        \begin{bmatrix}
            2&-1\\
            0&2
        \end{bmatrix}\\
                &=
        \begin{bmatrix}
            13&8\\
            8&5
        \end{bmatrix}
    .\end{align*}
    \begin{align*}
        A^2 &=
        \begin{bmatrix}
            1&3\\
            2&-1
        \end{bmatrix}
        \begin{bmatrix}
            1&3\\
            2&-1
        \end{bmatrix}
        =
        \begin{bmatrix}
            7&1\\
            0&7
        \end{bmatrix}
        \\
        B^2 &=
        \begin{bmatrix}
            2&-1\\
            0&2
        \end{bmatrix}
        \begin{bmatrix}
            2&-1\\
            0&2
        \end{bmatrix}
        =
        \begin{bmatrix}
            4&-4\\
            0&4
        \end{bmatrix}
        \\
        AB &=
        \begin{bmatrix}
            1&3\\
            2&-1
        \end{bmatrix}
        \begin{bmatrix}
            2&-1\\
            0&2
        \end{bmatrix}
        =
        \begin{bmatrix}
            2&5\\
            4&-4
        \end{bmatrix}
        \\
        2AB &= \begin{bmatrix} 4&10\\8&-8 \end{bmatrix} 
    .\end{align*}
    \[
        A^2+B^2+2AB = \begin{bmatrix} 15&6\\8&-3 \end{bmatrix}
    .\] 

\end{example}

\begin{note}
    \[
        (A+B)^2 \neq A^2+2AB+B^2
    .\] 
    \[
        (A+B)^2 = A^2+AB+BA+B^2
    .\] 
\end{note}

\begin{example}[$AC=BC$ does not imply $A=B$]
    \[
        A =
        \begin{bmatrix}
            1&3\\
            0&1
        \end{bmatrix},
        B =
        \begin{bmatrix}
            2&4\\
            2&3
        \end{bmatrix},
        C =
        \begin{bmatrix}
            1&-2\\
            -1&2
        \end{bmatrix}
    .\] 
    \begin{align*}
        AC &=
        \begin{bmatrix} -2&4\\-1&2 \end{bmatrix} \\
        BC &=
        \begin{bmatrix} -2&4\\-1&2 \end{bmatrix} 
    .\end{align*}
\end{example}

\newpage

\begin{example}
    \[
        A=
        \begin{bmatrix} 2&3&1\\5&4&-1 \end{bmatrix},
        B=
        \begin{bmatrix} 2&5&4 \end{bmatrix} 
    .\] 
    \[
        AB = 
        \begin{bmatrix} 
            2\times 2+3\times 5+4\times 1\\
            5\times 2+4\times 5-4\times 1
        \end{bmatrix} 
        =
        \begin{bmatrix} 23\\26 \end{bmatrix} 
    .\] 
    $BA \longrightarrow$ does not exist because number of columns in $B$ doesn't equal the number of rows in $A$
\end{example}
\hspace{1em}

The Matrix multiplication identity is called $I$.

\begin{example}
    \[
        \begin{bmatrix} 2&3\\4&5 \end{bmatrix} 
        \begin{bmatrix} 1&0\\0&1 \end{bmatrix} 
        =
        \begin{bmatrix} 2&3\\4&5 \end{bmatrix} 
    .\] 
    \[ AI_2=A .\] 
\end{example}

\begin{example}
    \[
        \begin{bmatrix} 1&0&0\\0&1&0\\0&0&1 \end{bmatrix} 
        \begin{bmatrix} 2&3\\4&5\\1&2 \end{bmatrix} 
        =
        \begin{bmatrix} 2&3\\4&5\\1&2 \end{bmatrix} 
    .\] 
    \[ I_3B=B .\] 
\end{example}

\begin{note}
    In $R^n$, $I_n$ is a matrix with ones on the diagonal and it is the multiplication identity.
\end{note}

\begin{itemize}
    \item $A(BC)=(AB)C$
    \item $A(B+C)=AB+AC$
    \item $k(AB)=(kA)B=A(kB)$ where ($k$ is a scalar)
    \item $A_{m\times n}I_n=A$
    \item $I_mA_{m\times n}=A$
    \item $A^n= A A \ldots A$
\end{itemize}

\subsection{Transpose of Matrix}

\begin{definition}[Matrix Transpose]
    Just interchange the matrix's rows and columns.
\end{definition}

\begin{example}
    \[
        A = \begin{bmatrix} 2&4&-5\\1&-3&2 \end{bmatrix} 
        \longrightarrow
        A^T=\begin{bmatrix} 2&1\\4&-3\\-5&2 \end{bmatrix} 
    .\] 
    \[
        B = \begin{bmatrix} 2\\4\\3 \end{bmatrix} 
        \longrightarrow
        B^T=\begin{bmatrix} 2&4&3 \end{bmatrix} 
    .\] 
\end{example}

\begin{example}[Find $(AB)^T$ and $B^TA^T$]
    \[
        A=\begin{bmatrix} 2&4&-5\\1&-3&2 \end{bmatrix},
        B=\begin{bmatrix} 2\\4\\3 \end{bmatrix} 
    .\]
    \begin{align*}
        AB &=
        \begin{bmatrix} 2&4&-5\\1&-3&2 \end{bmatrix}
        \begin{bmatrix} 2\\4\\3 \end{bmatrix}
        =
        \begin{bmatrix} 5\\-4 \end{bmatrix} \\
        (AB)^T &= \begin{bmatrix} 5&-4 \end{bmatrix} \\
        B^TA^T &=
        \begin{bmatrix} 2&4&3 \end{bmatrix} 
        \begin{bmatrix} 2&1\\4&-3\\-5&2 \end{bmatrix} 
        =
        \begin{bmatrix} 5&-4 \end{bmatrix} 
    .\end{align*}
\end{example}

\begin{note}
    \[
        (AB)^T=B^TA^T
    .\] 
\end{note}

\begin{itemize}
    \item $(ABC)^T=C^T(AB)^T=C^TB^TA^T$
    \item $ (A^T)^T=A $
    \item $(AT)^T=B^TA^T$
    \item $(A+B)^T=A^T+B^T$
    \item $ k(A)^T=(kA)^T $
\end{itemize}

\begin{example}[Find $AA^T$ and  $A^TA$]
    \begin{align*}
        A &=
        \begin{bmatrix} 2&4&-5\\1&-3&2 \end{bmatrix} \\
        AA^T &=
        \begin{bmatrix} 2&4&-5\\1&-3&2 \end{bmatrix} 
        \begin{bmatrix} 2&1\\4&-3\\-5&2 \end{bmatrix} 
        =
        \begin{bmatrix} 45&-20\\-20&14 \end{bmatrix} \\
        A^TA &=
        \begin{bmatrix} 2&1\\4&-3\\-5&2 \end{bmatrix} 
        \begin{bmatrix} 2&4&-5\\1&-3&2 \end{bmatrix} 
        =
        \begin{bmatrix} 
            5&5&-8\\
            5&25-26\\
            -8&-26&29
        \end{bmatrix} 
    .\end{align*}
\end{example}

\begin{note}
    \[
        AA^T \neq A^TA
    .\] 
\end{note}
\info{Both are square matrices.}
\info{Both are symmetric matrices.}
\info{$(AA^T)^T=AA^T$}

\subsection{The Trace of Matrix}
Only square matrices have a trace.

\begin{definition}
    \[
        Tr(A) = \text{sum of the diagonal elements}
    .\] 
\end{definition}

\[
    A =
    \begin{bmatrix}
        1&4&-5\\
        1&-3&7\\
        4&3&6\\
    \end{bmatrix}
    \longrightarrow
    Tr(A)=1+(-3)+6=4
.\] 

\begin{example}[Find $Tr(AB)$, $Tr(BA)$, and $Tr(A+B)$]
    \[
        A=
        \begin{bmatrix} 4&5\\2&-1 \end{bmatrix} 
        ,
        B=
        \begin{bmatrix} 2&-1\\-2&3 \end{bmatrix} 
    .\] 
    \[
        Tr(A)=3, Tr(B)=4, Tr(A)+Tr(B)=8
    .\] 
    \[
        A+B=\begin{bmatrix} 6&4\\0&2 \end{bmatrix}
        \longrightarrow
        Tr(A+B)=8
    .\] 
\end{example}

\begin{note}
    \[
        Tr(A+B)=Tr(A)+Tr(B)
    .\] 
\end{note}

\begin{example}[Find $2Tr(A)$, $Tr(2A)$, $Tr(AB)$, $Tr(BA)$]
    \[
        A=
        \begin{bmatrix} 4&5\\2&-1 \end{bmatrix} 
        ,
        B=
        \begin{bmatrix} 2&-1\\0&2 \end{bmatrix} 
    .\] 
    \[
        2Tr(A)=2\times 3=6
    .\] 
    \[
        2A=\begin{bmatrix} 8&6\\4&-2 \end{bmatrix}
        \longrightarrow
        Tr(2A)=6
    .\] 
    \[
        Tr(AB)=Tr(\begin{bmatrix} 8&2\\4&-4 \end{bmatrix} ) =4
    .\] 
    \[
        Tr(AB)=Tr(\begin{bmatrix} 6&7\\4&-2 \end{bmatrix} ) =4
    .\] 
\end{example}

\begin{note}
    \[
        \begin{rcases*}
            Tr(kA)=kTr(A)\\
            Tr(AB)=TR(BA)
        \end{rcases*}
        \longrightarrow
        \text{Always True}
    .\]
\end{note}

\[
    Tr(ABC)=Tr(CAB)=Tr(BCA)
.\] 

\subsubsection{Trace Properties}

\begin{itemize}
    \item $Tr(A)=\sum_{i=1}^n a_{i i} \rho=8$
    \item $Tr(A+B)=Tr(A)+Tr(B)$
    \item If $k$ is scalar, $Tr(kA)=k Tr(A)$
    \item $Tr(A B)=Tr(B A)$
    \item $Tr(A^T)=Tr(A)$
\end{itemize}

\subsection{Special Matrix Shapes}

\newcolumntype{M}{>{\begin{varwidth}{3cm}}l<{\end{varwidth}}} %M is for Maximal column
\begin{tabular}{Mlll}
    Row vector & $V_{1\times 3}=\begin{bmatrix} 2&4&1 \end{bmatrix}$ \\
    \\
    Column vector & $W_{2\times 1}=\begin{bmatrix}4\\5\end{bmatrix}$\\
    \\
    Upper triangular & $U_{3 \times 3}=\begin{bmatrix} 1&-1&2\\0&3&5\\0&0&-6 \end{bmatrix}$\\
    \\
    Lower triangular & $\begin{bmatrix} 4&0&0\\3&6&0\\9&7&-6 \end{bmatrix} $\\
    \\
    Diagonal Matrix & $D_{3\times 3}=\begin{bmatrix} 2&0&0\\0&3&0\\0&0&-6 \end{bmatrix} $\\
    \\
    Identity Matrix\\(A special case of the Diagonal matrix) & $U_3=\begin{bmatrix} 1&0&0\\0&1&0\\0&0&1 \end{bmatrix} $\\
    \\
    Symmetric Matrix & $A_{3\times 3}=\begin{bmatrix}1&2&-5\\2&4&5\\-3&5&0\end{bmatrix}$ & ($A^T=A$) &
    $\begin{array} {ccc} a_{12}=a_{21}\\ a_{13}=a_{31}\\ a_{23}=a_{32}\end{array}$
    \\
    \\
    Skew-Symmetric Matrix & $A_{3\times 3}=\begin{bmatrix}0&-2&-3\\2&0&5\\3&-5&0\end{bmatrix}$ & ($A^T=-A$) & 
    $\begin{array} {ccc} a_{12}=-a_{21}\\ a_{13}=-a_{31}\\ a_{23}=-a_{32}\end{array}$
\end{tabular}

\end{document}
